test

QuantumComputer3Qubits/Tests/TransformOperators.lean
@@ -1,1 +1,33 @@
 import QuantumComputer3Qubits.Formalization.TransformOperators
+import QuantumComputer3Qubits.Tests.StateExamples
+
+namespace Test_TransformOperators
+
+def id:OP.o1:=
+{
+  toFun(s: StateReg1) := s
+  map_add' := by aesop
+  map_smul' := by aesop
+}
+
+theorem idProp: ∀s: StateReg1, id s = s := by
+  simp [id]
+
+def not:OP.o1:=
+{
+  toFun(s: StateReg1) := fun x:Fin 2 =>
+        match x with
+        | 0 => s 1
+        | 1 => s 0
+  map_add' := by aesop
+  map_smul' := by aesop
+}
+
+theorem notProp: (not SE.s0 = SE.s1) ∧ (not SE.s1 = SE.s0) := by
+  simp [not]
+  aesop
+
+theorem test1:∀i: Fin 3, ∀s: StateReg1Ind i,
+              TO.o1_oi1 i id s = s := by
+  simp [TO.o1_oi1, LER.reg1i_reg1]
+  aesop
